Verified bubble sort

verification/fff.dfy
@@ -26,3 +26,46 @@ method average(a: array<int>) returns (avg: int)
   
   if (i == 0) {avg := -1;} else {avg := total/i;}
 }
+
+predicate sorted (a:array<int>, start:int, end:int)
+ requires a!=null
+ requires 0<=start<=end<=a.Length
+ reads a
+{
+ forall j,k:: start <= j < k < end ==> a[j]<=a[k]
+}
+
+method Bubble_sort(a: array<int>)
+requires a != null && a.Length > 1;
+modifies a;
+ensures sorted(a, 0, a.Length);
+{
+  var i := 0;
+  while (i < a.Length) 
+    invariant 0 <= i <= a.Length
+    invariant sorted(a, a.Length - i, a.Length)
+    invariant forall k :: 0 <= k < a.Length - i && i > 0 ==> a[k] <= a[a.Length -i]
+    decreases a.Length - i
+  {
+    var j := 0;
+    while (j < a.Length - i - 1) 
+      invariant 0 <= j <= a.Length - i - 1
+      invariant sorted(a, a.Length - i, a.Length)  
+      invariant forall k :: 0 <= k < a.Length - i && i > 0 ==> a[k] <= a[a.Length -i]
+      invariant forall k :: 0 <= k < j ==> a[k] <= a[j]
+      invariant i > 0 ==> a[j] <= a[a.Length - i]
+      decreases a.Length - i - 1 - j
+    {
+      if a[j] > a[j+1]
+      {
+        var temp := a[j];
+        a[j] := a[j+1];
+        a[j+1] := temp;
+      }
+      
+      j := j + 1;
+    }
+    
+    i := i + 1;
+  }
+}
